### Question2

yxu49 Yijiong Xu

wzhu8 Wenqiao Zhu


$L(\mu x)= \frac{1}{\sigma \sqrt[]{2\pi}}exp(\frac {-(x_{1j}-\mu_1 k)^2}{2\sigma^2})-\frac{1}{\sigma \sqrt[]{2\pi}}exp(\frac {-(x_{2j}-\mu_1k)^2}{2\sigma^2})-.....-\frac{1}{\sigma \sqrt[]{2\pi}}exp(\frac {-(x_{nj}-\mu_1k)^2}{2\sigma^2})$

$=\frac{1}{\sigma \sqrt[]{2\pi}}exp-(\frac {(x_{1j}-\mu_1k)^2+.....+(x_{nj}-\mu_1k)^2}{2\sigma^2})$

$L_nL(\mu_1k)=(\frac {(x_{1j}-\mu_1k)^2+.....+(x_{nj}-\mu_1k)^2}{2\sigma^2})-L_n\sigma\sqrt[]{2\pi}$

$\frac {dL_nL(\mu_1k)}{d\mu_1k}=\frac {-2(x_{1j}-\mu_1k)-.....-2(x_{nj}-\mu_1k)}{2\sigma^2}$

$=\frac {n\mu_1k-(x_{1j}+.....+x_{nj})}{\sigma^2}=0$

Then we  can get $\mu_1k= \frac{x_{ij}+x_{nj}} {n}=\frac {\sum_{i=0}^{n}xij}{n}$